Use difference lists for faster writer monad

theories/compiler/compile.v
@@ -20,6 +20,8 @@ Require Import Wasm.numerics.
 
 From RichWasm Require term.
 From RichWasm Require Import typing.
+Require RichWasm.util.dlist.
+Import dlist.Notation.
 From RichWasm.compiler Require Import numerics util.
 
 Module R := term.
@@ -32,7 +34,7 @@ Definition size_ctx := list W.immediate.
 Definition wlocal_ctx := list W.value_type.
 
 Record wst (A : Type) :=
-  { un_wst : stateT wlocal_ctx (writerT (@Monoid_list_app W.basic_instruction) (sum err)) A }.
+  { un_wst : stateT wlocal_ctx (writerT (@dlist.Monoid_dlist W.basic_instruction) (sum err)) A }.
 
 Arguments Build_wst {A} _.
 Arguments un_wst {A} _.
@@ -51,7 +53,7 @@ Global Instance MonadState_wst : MonadState wlocal_ctx wst :=
   { get := Build_wst get;
     put := fun x => Build_wst (put x) }.
 
-Global Instance MonadWriter_wst : MonadWriter (@Monoid_list_app W.basic_instruction) wst :=
+Global Instance MonadWriter_wst : MonadWriter (@dlist.Monoid_dlist W.basic_instruction) wst :=
   { tell := fun x => Build_wst (tell x);
     listen := fun _ c => Build_wst (listen (un_wst c));
     (* Work around broken implementation of `pass` in ExtLib.
@@ -66,11 +68,11 @@ Definition lift_err {A} (c : err + A) : wst A :=
 Definition run_compiler (c : wst unit) (wl : wlocal_ctx) : err + wlocal_ctx * list W.basic_instruction :=
   match runWriterT (runStateT (un_wst c) wl) with
   | inl e => inl e
-  | inr x => inr (snd (PPair.pfst x), PPair.psnd x)
+  | inr x => inr (snd (PPair.pfst x), dlist.to_list (PPair.psnd x))
   end.
 
-Definition capture {A} (c : wst A) : wst (A * list W.basic_instruction) :=
-  censor (const []) (listen c).
+Definition capture {A} (c : wst A) : wst (A * dlist.dlist W.basic_instruction) :=
+  censor (const []%DL) (listen c).
 
 Record compiler_mod_ctx := {
   mem_gc : W.immediate;
@@ -206,13 +208,13 @@ Definition if_gc_bit_set {A} {B}
 : wst (A * B) :=
   tell [W.BI_const (W.VAL_int32 (Wasm_int.int_of_Z numerics.i32m 1%Z));
         W.BI_binop W.T_i32 (W.Binop_i W.BOI_and);
-        W.BI_testop W.T_i32 W.TO_eqz];;
+        W.BI_testop W.T_i32 W.TO_eqz]%DL;;
   '(x, lin_es) <- capture (lin_branch);;
   '(y, gc_es) <- capture (gc_branch);;
-  tell [W.BI_if (W.Tf ins outs) lin_es gc_es];;
+  tell [W.BI_if (W.Tf ins outs) (dlist.to_list lin_es) (dlist.to_list gc_es)]%DL;;
   ret (x, y).
 
-Definition unset_gc_bit :=
+Definition unset_gc_bit : dlist.dlist W.basic_instruction :=
   [W.BI_const (W.VAL_int32 (Wasm_int.int_of_Z numerics.i32m 1%Z));
    W.BI_binop W.T_i32 (W.Binop_i W.BOI_sub)].
 
@@ -220,7 +222,8 @@ Fixpoint loads'
   (mem: W.immediate)
   (base_ptr_var: W.immediate)
   (off: W.static_offset)
-  (tys: list W.value_type) :=
+  (tys: list W.value_type)
+: dlist.dlist W.basic_instruction :=
   match tys with
   | [] => []
   | ty :: tys =>
@@ -229,14 +232,15 @@ Fixpoint loads'
       loads' base_ptr_var mem (off + N.of_nat (operations.length_t ty))%N tys
   end.
 
-Definition loads mem base_ptr_var tys :=
+Definition loads mem base_ptr_var tys : dlist.dlist W.basic_instruction :=
   loads' mem base_ptr_var 0%N tys.
 
 Fixpoint loc_stores'
   (base_ptr_var: W.immediate)
   (mem: W.immediate)
   (off: W.static_offset)
-  (val_var_tys: list (W.immediate * W.value_type)) :=
+  (val_var_tys: list (W.immediate * W.value_type))
+: dlist.dlist W.basic_instruction :=
   match val_var_tys with
   | [] => []
   | (val_var, ty) :: val_var_tys =>
@@ -246,11 +250,11 @@ Fixpoint loc_stores'
       loc_stores' base_ptr_var mem (off + N.of_nat (operations.length_t ty))%N val_var_tys
   end.
 
-Definition loc_stores base_ptr_var mem val_var_tys : list W.basic_instruction :=
+Definition loc_stores base_ptr_var mem val_var_tys : dlist.dlist W.basic_instruction :=
   loc_stores' base_ptr_var mem 0%N val_var_tys.
 
 Definition stores base_ptr_var mem (val_vars: list W.immediate) (tys: list W.value_type)
-  : list W.basic_instruction :=
+  : dlist.dlist W.basic_instruction :=
   loc_stores base_ptr_var mem (zip val_vars tys).
 
 Inductive VarScope :=
@@ -299,9 +303,9 @@ Definition for_gc_ref_vars (scope : VarScope) (vars : list W.immediate) (m : wst
   iterM
     (fun var =>
        let '(get, set) := scope_get_set scope in
-       tell [get var];;
+       tell [get var]%DL;;
        if_gc_bit_set [W.T_i32] [W.T_i32] m (ret tt);;
-       tell [set var])
+       tell [set var]%DL)
     vars.
 
 Section Mod.
@@ -313,19 +317,19 @@ Section Mod.
   Definition tagged_store
     (base_ptr: W.immediate)
     (arg_vars: list W.immediate)
-    (offset_instrs: list W.basic_instruction)
+    (offset_instrs: dlist.dlist W.basic_instruction)
     (ty: R.Typ)
     : wst unit :=
     tell [W.BI_tee_local base_ptr;
-          W.BI_get_local base_ptr];;
+          W.BI_get_local base_ptr]%DL;;
     let tys := compile_typ ty in
     if_gc_bit_set [] []
-      (tell [W.BI_get_local base_ptr];;
+      (tell [W.BI_get_local base_ptr]%DL;;
        tell unset_gc_bit;;
        tell offset_instrs;;
-       tell [W.BI_set_local base_ptr];;
+       tell [W.BI_set_local base_ptr]%DL;;
        tell (stores base_ptr mctx.(mem_gc) arg_vars tys))
-      (tell [W.BI_get_local base_ptr];;
+      (tell [W.BI_get_local base_ptr]%DL;;
        tell offset_instrs;;
        tell (stores base_ptr mctx.(mem_lin) arg_vars tys));;
     ret tt.
@@ -357,7 +361,7 @@ Section Mod.
 
     Definition walloc_args (tys: list W.value_type) : wst (list W.immediate) :=
       vars <- wallocs tys;;
-      tell (map W.BI_set_local vars);;
+      tell (dlist.of_list (map W.BI_set_local vars));;
       ret vars.
 
     Definition walloc_rvalue (ty : R.Typ) : wst W.immediate :=
@@ -381,35 +385,35 @@ Section Mod.
 
     Definition gc_loads
       (ref_var: W.immediate)
-      (offset_instrs: list W.basic_instruction)
+      (offset_instrs: dlist.dlist W.basic_instruction)
       (tys: list W.value_type)
     : wst unit :=
       base_ptr_var <- walloc W.T_i32;;
-      tell [W.BI_get_local ref_var];;
+      tell [W.BI_get_local ref_var]%DL;;
       tell unset_gc_bit;;
       tell offset_instrs;;
       tell [W.BI_binop W.T_i32 (W.Binop_i W.BOI_add);
-            W.BI_set_local base_ptr_var];;
+            W.BI_set_local base_ptr_var]%DL;;
       tell (loads mctx.(mem_gc) base_ptr_var tys).
 
     Definition lin_loads
       (ref_var: W.immediate)
-      (offset_instrs: list W.basic_instruction)
+      (offset_instrs: dlist.dlist W.basic_instruction)
       (tys: list W.value_type)
     : wst unit :=
       base_ptr_var <- walloc W.T_i32;;
-      tell [W.BI_get_local ref_var];;
+      tell [W.BI_get_local ref_var]%DL;;
       tell offset_instrs;;
       tell [W.BI_binop W.T_i32 (W.Binop_i W.BOI_add);
-            W.BI_set_local base_ptr_var];;
+            W.BI_set_local base_ptr_var]%DL;;
       tell (loads mctx.(mem_lin) base_ptr_var tys).
 
     Definition tagged_loads
       (base_ptr: W.immediate)
-      (offset_instrs: list W.basic_instruction)
+      (offset_instrs: dlist.dlist W.basic_instruction)
       (tys: list W.value_type)
       : wst unit :=
-      tell [W.BI_get_local base_ptr];;
+      tell [W.BI_get_local base_ptr]%DL;;
       if_gc_bit_set [] tys
         (gc_loads base_ptr offset_instrs tys)
         (lin_loads base_ptr offset_instrs tys);;
@@ -417,19 +421,19 @@ Section Mod.
 
     Definition tagged_load
       (base_ptr: W.immediate)
-      (offset_instrs: list W.basic_instruction)
+      (offset_instrs: dlist.dlist W.basic_instruction)
       (ty: R.Typ)
     : wst unit :=
       let tys := compile_typ ty in
       tagged_loads base_ptr offset_instrs tys.
 
-    Definition tagged_store' (offset_instrs : list W.basic_instruction) (ty : R.Typ) : wst unit :=
+    Definition tagged_store' (offset_instrs : dlist.dlist W.basic_instruction) (ty : R.Typ) : wst unit :=
       let tys := compile_typ ty in
       arg_vars <- walloc_args tys;;
       base_ptr_var <- walloc W.T_i32;;
       tagged_store base_ptr_var arg_vars offset_instrs ty.
 
-    Definition get_i64_local (loc : W.immediate) : list W.basic_instruction :=
+    Definition get_i64_local (loc : W.immediate) : dlist.dlist W.basic_instruction :=
       [ W.BI_get_local loc;
         W.BI_cvtop W.T_i32 W.CVO_reinterpret W.T_i64 None;
         W.BI_get_local (loc + 1);
@@ -448,9 +452,9 @@ Section Mod.
              W.BI_get_local tmp;
              W.BI_const (W.VAL_int64 (Wasm_int.int_of_Z i64m 32));
              W.BI_binop W.T_i64 (W.Binop_i W.BOI_rotr);
-             W.BI_set_local (loc + 1) ].
+             W.BI_set_local (loc + 1) ]%DL.
 
-    Definition numtyp_gets (nτ: R.NumType) (loc: nat) : list W.basic_instruction :=
+    Definition numtyp_gets (nτ: R.NumType) (loc: nat) : dlist.dlist W.basic_instruction :=
       match nτ with
       | R.Int s R.i32 => [ W.BI_get_local loc ]
       | R.Float R.f32 =>
@@ -464,17 +468,17 @@ Section Mod.
 
     Definition numtyp_sets (nτ: R.NumType) (loc: nat) : wst unit :=
       match nτ with
-      | R.Int s R.i32 => tell [W.BI_set_local loc]
+      | R.Int s R.i32 => tell [W.BI_set_local loc]%DL
       | R.Float R.f32 =>
           tell [W.BI_cvtop W.T_f32 W.CVO_reinterpret W.T_i32 None;
-                W.BI_set_local loc]
+                W.BI_set_local loc]%DL
       | R.Int s R.i64 => set_i64_local loc
       | R.Float R.f64 =>
-          tell [W.BI_cvtop W.T_f64 W.CVO_reinterpret W.T_i64 None];;
+          tell [W.BI_cvtop W.T_f64 W.CVO_reinterpret W.T_i64 None]%DL;;
           set_i64_local loc
       end.
 
-    Fixpoint local_gets (τ: R.Typ) (loc: nat) : list W.basic_instruction :=
+    Fixpoint local_gets (τ: R.Typ) (loc: nat) : dlist.dlist W.basic_instruction :=
       match τ with
       | R.Num nτ =>
           numtyp_gets nτ loc
@@ -489,8 +493,8 @@ Section Mod.
                 let sz := words_typ τ0 in
                 let es := local_gets τ0 loc in
                 let es' := loop τs0' (loc + sz) in
-                es ++ es'
-            | [] => []
+                (es ++ es')%DL
+            | [] => []%DL
             end in
           loop τs loc
       | R.CoderefT χ =>
@@ -514,7 +518,7 @@ Section Mod.
       | R.Num nτ =>
           numtyp_sets nτ loc
       | R.TVar α =>
-          tell [W.BI_set_local loc]
+          tell [W.BI_set_local loc]%DL
       | R.Unit =>
           ret tt
       | R.ProdT τs =>
@@ -528,11 +532,11 @@ Section Mod.
             end in
           loop τs loc
       | R.CoderefT χ =>
-          tell [W.BI_set_local loc]
+          tell [W.BI_set_local loc]%DL
       | R.Rec q τ =>
           local_sets τ loc
       | R.PtrT ℓ =>
-          tell [W.BI_set_local loc]
+          tell [W.BI_set_local loc]%DL
       | R.ExLoc q τ =>
           local_sets τ loc
       | R.OwnR ℓ =>
@@ -540,7 +544,7 @@ Section Mod.
       | R.CapT cap ℓ ψ =>
           ret tt
       | R.RefT cap ℓ ψ =>
-          tell [W.BI_set_local loc]
+          tell [W.BI_set_local loc]%DL
       end.
 
     Definition save_stack (tys : list R.Typ) : wst W.immediate :=
@@ -548,69 +552,69 @@ Section Mod.
       local_sets (R.ProdT tys) idx;;
       ret idx.
 
-    Definition restore_stack (tys : list R.Typ) (idx : W.immediate) : list W.basic_instruction :=
+    Definition restore_stack (tys : list R.Typ) (idx : W.immediate) : dlist.dlist W.basic_instruction :=
       local_gets (R.ProdT tys) idx.
 
-    Fixpoint compile_sz (sz : R.Size) : err + list W.basic_instruction :=
+    Fixpoint compile_sz (sz : R.Size) : err + dlist.dlist W.basic_instruction :=
       match sz with
       | R.SizeVar σ =>
         local_idx <- err_opt (lookup σ sz_locs) ("sz " ++ pretty σ ++ " not found in sz_local_map");;
-        inr [W.BI_get_local local_idx]
+        inr [W.BI_get_local local_idx]%DL
       | R.SizePlus sz1 sz2 =>
         e1 <- compile_sz sz1;;
         e2 <- compile_sz sz2;;
-        inr (e1 ++ e2 ++ [W.BI_binop W.T_i32 (W.Binop_i W.BOI_add)])
+        inr (e1 ++ e2 ++ [W.BI_binop W.T_i32 (W.Binop_i W.BOI_add)])%DL
       | R.SizeConst c =>
-        inr [W.BI_const (W.VAL_int32 (Wasm_int.int_of_Z i32m (Z.of_nat c)))]
+        inr [W.BI_const (W.VAL_int32 (Wasm_int.int_of_Z i32m (Z.of_nat c)))]%DL
       end.
 
-    Definition compile_ind (ind: R.Index) : err + list W.basic_instruction :=
+    Definition compile_ind (ind: R.Index) : err + dlist.dlist W.basic_instruction :=
       match ind with
       | R.SizeI sz => compile_sz sz
       | R.LocI _
       | R.QualI _
-      | R.TypI _ => ret []
+      | R.TypI _ => inr []%DL
       end.
 
-    Definition compile_inds (inds: list R.Index) : err + list W.basic_instruction :=
-      flatten <$> mapT compile_ind inds.
+    Definition compile_inds (inds: list R.Index) : err + dlist.dlist W.basic_instruction :=
+      dlist.concat <$> mapT compile_ind inds.
 
     Fixpoint compile_instr (instr: R.instr TyAnn) : wst unit :=
       match instr with
-      | R.INumConst _ num_type num => tell [W.BI_const (compile_num num_type num)]
+      | R.INumConst _ num_type num => tell [W.BI_const (compile_num num_type num)]%DL
       | R.IUnit _ => ret tt
       | R.INum ann ni =>
           e <- lift_err (compile_num_instr ni);;
-          tell [e]
-      | R.IUnreachable (R.Arrow targs trets, _) => tell [W.BI_unreachable]
-      | R.INop (R.Arrow targs trets, _) => tell [W.BI_nop]
+          tell [e]%DL
+      | R.IUnreachable (R.Arrow targs trets, _) => tell [W.BI_unreachable]%DL
+      | R.INop (R.Arrow targs trets, _) => tell [W.BI_nop]%DL
       | R.IDrop (R.Arrow targs trets, LSig L _) =>
           match targs with
           | [t_drop] =>
               let wasm_typ := compile_typ t_drop in
               base <- save_stack [t_drop];;
               let ref_vars := map (Nat.add base) (ref_indices LMNative t_drop) in
-              for_gc_ref_vars VSLocal ref_vars (tell [W.BI_call mctx.(unregisterroot)]);;
+              for_gc_ref_vars VSLocal ref_vars (tell [W.BI_call mctx.(unregisterroot)]%DL);;
               tell (restore_stack [t_drop] base);;
-              tell (map (const W.BI_drop) wasm_typ)
+              tell (dlist.of_list (map (const W.BI_drop) wasm_typ))
           | _ => raise (Err "drop should consume exactly one value")
           end
       | R.IBlock (R.Arrow targs trets, _) ta _ es =>
           let ta' := compile_arrow_type ta in
           '(_, es') <- capture (forT es compile_instr);;
-          tell [W.BI_block ta' es']
+          tell [W.BI_block ta' (dlist.to_list es')]%DL
       | R.ILoop (R.Arrow targs trets, _) arrow es =>
           let ft := compile_arrow_type arrow in
           '(_, es') <- capture (forT es compile_instr);;
-          tell [W.BI_loop ft es']
+          tell [W.BI_loop ft (dlist.to_list es')]%DL
       | R.IIte (R.Arrow targs trets, _) arrow _ ets efs =>
           let ft := compile_arrow_type arrow in
           '(_, ets') <- capture (forT ets compile_instr);;
           '(_, efs') <- capture (forT efs compile_instr);;
-          tell [W.BI_if ft ets' efs']
-      | R.IBr (R.Arrow targs trets, _) x => tell [W.BI_br x]
-      | R.IBrIf (R.Arrow targs trets, _) x => tell [W.BI_br_if x]
-      | R.IBrTable (R.Arrow targs trets, _) x x0 => tell [W.BI_br_table x x0]
+          tell [W.BI_if ft (dlist.to_list ets') (dlist.to_list efs')]%DL
+      | R.IBr (R.Arrow targs trets, _) x => tell [W.BI_br x]%DL
+      | R.IBrIf (R.Arrow targs trets, _) x => tell [W.BI_br_if x]%DL
+      | R.IBrTable (R.Arrow targs trets, _) x x0 => tell [W.BI_br_table x x0]%DL
       | R.IRet (R.Arrow targs trets, _) =>
           let ret_ty' := ssrfun.Option.default [] F.(rettyp) in
           let rdropped := take (length targs - length ret_ty') targs in
@@ -618,53 +622,53 @@ Section Mod.
           idx_ret <- save_stack ret_ty';;
           idx_dropped <- save_stack rdropped;;
           let ref_vars := map (Nat.add idx_dropped) (flat_map (ref_indices LMNative) rdropped) in
-          for_gc_ref_vars VSLocal ref_vars (tell [W.BI_call mctx.(unregisterroot)]);;
+          for_gc_ref_vars VSLocal ref_vars (tell [W.BI_call mctx.(unregisterroot)]%DL);;
           tell (restore_stack ret_ty' idx_ret);;
-          tell [W.BI_return]
+          tell [W.BI_return]%DL
       | R.IGetLocal (R.Arrow targs trets, LSig L _) idx _ =>
           '(base, τ) <- lift_err (local_layout L 0 idx);;
           tell (local_gets τ base);;
           'i <- save_stack [τ];;
           let ref_vars := map (Nat.add i) (ref_indices LMNative τ) in
-          for_gc_ref_vars VSLocal ref_vars (tell [W.BI_call mctx.(duproot)]);;
+          for_gc_ref_vars VSLocal ref_vars (tell [W.BI_call mctx.(duproot)]%DL);;
           tell (restore_stack [τ] i)
       | R.ISetLocal (R.Arrow targs trets, LSig L _) idx =>
           '(base, τ) <- lift_err (local_layout L 0 idx);;
           let ref_vars := map (Nat.add base) (ref_indices LMWords τ) in
-          for_gc_ref_vars VSLocal ref_vars (tell [W.BI_call mctx.(unregisterroot)]);;
+          for_gc_ref_vars VSLocal ref_vars (tell [W.BI_call mctx.(unregisterroot)]%DL);;
           local_sets τ base
       | R.IGetGlobal _ i =>
           '(i', ty) <- lift_err (err_opt (global_layout C.(global) i) "invalid global index");;
-          tell (imap (fun j _ => W.BI_get_global (i' + j)) (compile_typ ty));;
+          tell (dlist.of_list (imap (fun j _ => W.BI_get_global (i' + j)) (compile_typ ty)));;
           j <- save_stack [ty];;
           let ref_vars := map (Nat.add j) (ref_indices LMNative ty) in
-          for_gc_ref_vars VSLocal ref_vars (tell [W.BI_call mctx.(duproot)]);;
+          for_gc_ref_vars VSLocal ref_vars (tell [W.BI_call mctx.(duproot)]%DL);;
           tell (restore_stack [ty] i)
       | R.ISetGlobal _ i =>
           '(i', ty) <- lift_err (err_opt (global_layout C.(global) i) "invalid global index");;
           let ref_vars := map (Nat.add i') (ref_indices LMNative ty) in
-          for_gc_ref_vars VSGlobal ref_vars (tell [W.BI_call mctx.(unregisterroot)]);;
-          tell (imap (fun j _ => W.BI_set_global (i' + j)) (compile_typ ty))
+          for_gc_ref_vars VSGlobal ref_vars (tell [W.BI_call mctx.(unregisterroot)]%DL);;
+          tell (dlist.of_list (imap (fun j _ => W.BI_set_global (i' + j)) (compile_typ ty)))
       | R.ICoderef (R.Arrow targs trets, _) idx =>
           tell [W.BI_const (W.VAL_int32 (Wasm_int.int_of_Z i32m (Z.of_nat idx)));
                 W.BI_get_global mctx.(coderef_offset);
-                W.BI_binop W.T_i32 (W.Binop_i W.BOI_add)]
+                W.BI_binop W.T_i32 (W.Binop_i W.BOI_add)]%DL
       | R.ICallIndirect (R.Arrow targs trets, _) inds =>
           stk <- save_stack targs;;
           es <- lift_err (compile_inds inds);;
           tell es;;
           tell (restore_stack targs stk);;
-          tell [W.BI_call_indirect mctx.(fn_tab)]
+          tell [W.BI_call_indirect mctx.(fn_tab)]%DL
       | R.ICall (R.Arrow targs trets, _) fidx inds =>
           stk <- save_stack targs;;
           es <- lift_err (compile_inds inds);;
           tell es;;
           tell (restore_stack targs stk);;
-          tell [W.BI_call fidx]
+          tell [W.BI_call fidx]%DL
       | R.IMemUnpack _ ta tl es =>
           let ta' := compile_arrow_type ta in
           '(_, es') <- capture (forT es compile_instr);;
-          tell [W.BI_block ta' es']
+          tell [W.BI_block ta' (dlist.to_list es')]%DL
       | R.IStructMalloc (R.Arrow targs trets, _) szs q =>
           (* TODO: registerroot on the new address;
                    unregisterroot if any field is GC ref being put into GC struct *)
@@ -676,21 +680,21 @@ Section Mod.
           raise Todo
       | R.IStructFree (R.Arrow targs trets, _) =>
           (* TODO: unregisterroot fields that may be refs to GC if this struct is MM *)
-          tell [W.BI_call mctx.(free)]
+          tell [W.BI_call mctx.(free)]%DL
       | R.IStructGet (R.Arrow from to, _) n =>
           base_ref <- walloc W.T_i32;;
           fields <- lift_err (get_struct_field_types from 0);;
           field_typ <- lift_err (err_opt (list_lookup 0 to) "struct.get: cannot find output val type");;
           offset_sz <- lift_err (struct_field_offset fields n);;
           offset_es <- lift_err (compile_sz offset_sz);;
-          tell [W.BI_tee_local base_ref];;
+          tell [W.BI_tee_local base_ref]%DL;;
           tagged_load base_ref offset_es field_typ;;
           stk <- save_stack [field_typ];;
-          tell [W.BI_get_local base_ref];;
+          tell [W.BI_get_local base_ref]%DL;;
           let ref_vars := map (Nat.add stk) (ref_indices LMNative field_typ) in
           if_gc_bit_set [] []
-            (for_gc_ref_vars VSLocal ref_vars (tell [W.BI_call mctx.(registerroot)]))
-            (for_gc_ref_vars VSLocal ref_vars (tell [W.BI_call mctx.(duproot)]));;
+            (for_gc_ref_vars VSLocal ref_vars (tell [W.BI_call mctx.(registerroot)]%DL))
+            (for_gc_ref_vars VSLocal ref_vars (tell [W.BI_call mctx.(duproot)]%DL));;
           tell (restore_stack [field_typ] stk)
       | R.IStructSet (R.Arrow from to, _) n =>
           base_ref <- walloc W.T_i32;;
@@ -700,7 +704,7 @@ Section Mod.
           offset_sz <- lift_err (struct_field_offset fields n);;
           offset_es <- lift_err (compile_sz offset_sz);;
 
-          tell [W.BI_tee_local base_ref];;
+          tell [W.BI_tee_local base_ref]%DL;;
           if_gc_bit_set [] []
             (ret tt)
             (let tys := compile_typ field_typ in
@@ -708,18 +712,18 @@ Section Mod.
              old_stk_var <- save_stack [field_typ];;
              let old_ref_vars := map (Nat.add old_stk_var) (ref_indices LMNative field_typ) in
              for_gc_ref_vars VSLocal old_ref_vars
-               (tell [W.BI_call mctx.(unregisterroot)]));;
+               (tell [W.BI_call mctx.(unregisterroot)]%DL));;
 
-          tell [W.BI_get_local base_ref];;
+          tell [W.BI_get_local base_ref]%DL;;
           if_gc_bit_set [] []
             (new_stk_var <- save_stack [val_typ];;
              let new_ref_vars := map (Nat.add new_stk_var) (ref_indices LMNative val_typ) in
              for_gc_ref_vars VSLocal new_ref_vars
-               (tell [W.BI_load mctx.(mem_gc) W.T_i32 None 0%N 0%N]);;
+               (tell [W.BI_load mctx.(mem_gc) W.T_i32 None 0%N 0%N]%DL);;
              tell (restore_stack [val_typ] new_stk_var))
             (ret tt);;
 
-          tell [W.BI_get_local base_ref];;
+          tell [W.BI_get_local base_ref]%DL;;
           tagged_store' offset_es val_typ
       | R.IStructSwap (R.Arrow from to, _) n =>
           (* TODO: registerroot if GC struct *)
@@ -791,21 +795,22 @@ Section Mod.
           base_local <- walloc W.T_i32;;
           let words := words_typ elem_typ in
           tell [W.BI_set_local idx_local;
-                W.BI_set_local base_local];;
+                W.BI_set_local base_local]%DL;;
           tagged_load
             base_local
             [W.BI_const (W.VAL_int32 (Wasm_int.int_of_Z i32m 0))]
             (R.Num (R.Int R.U R.i32));;
           tell [W.BI_get_local idx_local;
-                W.BI_relop W.T_i32 (W.Relop_i (W.ROI_lt (W.SX_U)))];;
+                W.BI_relop W.T_i32 (W.Relop_i (W.ROI_lt (W.SX_U)))]%DL;;
           let compute_offset :=
             [W.BI_get_local idx_local;
              W.BI_const (W.VAL_int32 (Wasm_int.int_of_Z i32m (Z.of_nat words)));
              W.BI_binop W.T_i32 (W.Binop_i W.BOI_mul);
              W.BI_const (W.VAL_int32 (Wasm_int.int_of_Z i32m 4)); (* skip header length word *)
-             W.BI_binop W.T_i32 (W.Binop_i W.BOI_add)] in
+             W.BI_binop W.T_i32 (W.Binop_i W.BOI_add)]%DL in
           '(_, read_es) <- capture (tagged_load base_local compute_offset elem_typ);;
-          tell [W.BI_if (W.Tf [] elem_shape) read_es [W.BI_unreachable]]
+          let e := W.BI_if (W.Tf [] elem_shape) (dlist.to_list read_es) [W.BI_unreachable] in
+          tell [e]%DL
       | R.IArraySet (R.Arrow from to, _) =>
           (* TODO: unregisterroot if GC array;
                    duproot a bunch of times if MM array *)
