theories/util/dlist.v
@@ -1,0 +1,53 @@
+Require Import Coq.Program.Basics.
+Require Import Coq.Lists.List.
+
+Require Import ExtLib.Structures.Monoid.
+
+Record dlist A := { apply_dlist : list A -> list A }.
+
+Arguments Build_dlist {A} _.
+Arguments apply_dlist {A} _.
+
+Definition empty {A} : dlist A :=
+  Build_dlist id.
+
+Definition singleton {A} (x : A) : dlist A :=
+  Build_dlist (cons x).
+
+Definition cons {A} (x : A) (xs : dlist A) : dlist A :=
+  Build_dlist (compose (cons x) (apply_dlist xs)).
+
+Definition append {A} (xs : dlist A) (ys : dlist A) : dlist A :=
+  Build_dlist (compose (apply_dlist xs) (apply_dlist ys)).
+
+Definition concat {A} (xs : list (dlist A)) : dlist A :=
+  fold_right append empty xs.
+
+Definition of_list {A} (xs : list A) : dlist A :=
+  Build_dlist (app xs).
+
+Definition to_list {A} (xs : dlist A) : list A :=
+  apply_dlist xs nil.
+
+Definition Monoid_dlist {A} : Monoid (dlist A) :=
+  {| monoid_plus := append;
+     monoid_unit := empty |}.
+
+Module Notation.
+
+  Declare Scope dlist_scope.
+  Delimit Scope dlist_scope with DL.
+  Bind Scope dlist_scope with dlist.
+  Local Open Scope dlist_scope.
+
+  Infix "::" := cons : dlist_scope.
+
+  Infix "++" := append : dlist_scope.
+
+  Notation "[ ]" := empty : dlist_scope.
+
+  Notation "[ x ]" := (x :: []) : dlist_scope.
+
+  Notation "[ x1 ; x2 ; .. ; xn ]" := (x1 :: x2 :: .. [xn] ..) : dlist_scope.
+
+End Notation.
